Renamed lemmas and theorems

src/Operational.thy
@@ -84,61 +84,53 @@ lemma operational_semantics_trans_generalized:
   shows "\<C>\<^sub>1 \<hookrightarrow>\<^bsup>n + m\<^esup> \<C>\<^sub>3"
   by (metis (no_types, hide_lams) assms(1) assms(2) relcompp.relcompI relpowp_add)
 
-(* TODO *)
+(*
 inductive operational_semantics_simlstep :: "config \<Rightarrow> config \<Rightarrow> bool" ("_ \<hookrightarrow>\<^sub>\<nabla> _" 70) where
   "(\<Gamma>\<^sub>1, n \<turnstile> [] \<triangleright> \<Phi>\<^sub>1) \<hookrightarrow>\<^sup>+\<^sup>+ (\<Gamma>, n + 1 \<turnstile> [] \<triangleright> \<Phi>\<^sub>2) \<Longrightarrow>
    \<Psi>\<^sub>1 = [] \<Longrightarrow>
    \<Psi>\<^sub>2 = [] \<Longrightarrow>
    n' = Suc n \<Longrightarrow>
    (\<Gamma>\<^sub>1, n \<turnstile> \<Psi>\<^sub>1 \<triangleright> \<Phi>\<^sub>1) \<hookrightarrow>\<^sub>\<nabla> (\<Gamma>, n' \<turnstile> \<Psi>\<^sub>2 \<triangleright> \<Phi>\<^sub>2)"
+*)
 
-abbreviation Fnext_solve :: "config \<Rightarrow> config set" ("\<F>\<^sub>n\<^sub>e\<^sub>x\<^sub>t _") where
-  "\<F>\<^sub>n\<^sub>e\<^sub>x\<^sub>t \<S> \<equiv> { \<S>'. \<S> \<hookrightarrow> \<S>' }"
+abbreviation Cnext_solve :: "config \<Rightarrow> config set" ("\<C>\<^sub>n\<^sub>e\<^sub>x\<^sub>t _") where
+  "\<C>\<^sub>n\<^sub>e\<^sub>x\<^sub>t \<S> \<equiv> { \<S>'. \<S> \<hookrightarrow> \<S>' }"
 
-(* Is \<F>\<^sub>n\<^sub>e\<^sub>x\<^sub>t complete enough to have equality ? *)
-lemma Fnext_solve_instant:
-  shows "\<F>\<^sub>n\<^sub>e\<^sub>x\<^sub>t (\<Gamma>, n \<turnstile> [] \<triangleright> \<Phi>)
+lemma Cnext_solve_instant:
+  shows "\<C>\<^sub>n\<^sub>e\<^sub>x\<^sub>t (\<Gamma>, n \<turnstile> [] \<triangleright> \<Phi>)
           \<supseteq> { \<Gamma>, Suc n \<turnstile> \<Phi> \<triangleright> [] }"
   by (simp add: operational_semantics_step.simps operational_semantics_intro.instant_i)
 
-lemma Fnext_compose : "(\<F>\<^sub>n\<^sub>e\<^sub>x\<^sub>t \<S>) = { \<S>'. \<S> \<hookrightarrow>\<^sub>i \<S>' } \<union> { \<S>'. \<S> \<hookrightarrow>\<^sub>e \<S>' }"
-  oops
-
-(*
-lemma Fnext_empty : "{ \<S>'. \<exists> \<Gamma>' \<Phi>'.  \<Gamma>, n \<turnstile> [] \<triangleright> \<Phi> \<hookrightarrow>\<^sub>e \<Gamma>', Suc n \<turnstile> [] \<triangleright> \<Phi>' \<and> \<Gamma>', Suc n \<turnstile> [] \<triangleright> \<Phi>' = S'} = {}"    
-  sorry
-*)
-
-lemma Fnext_solve_sporadic:
-  shows "\<F>\<^sub>n\<^sub>e\<^sub>x\<^sub>t (\<Gamma>, n \<turnstile> (K sporadic \<tau>) # \<Psi> \<triangleright> \<Phi>)
+lemma Cnext_solve_sporadic:
+  shows "\<C>\<^sub>n\<^sub>e\<^sub>x\<^sub>t (\<Gamma>, n \<turnstile> (K sporadic \<tau>) # \<Psi> \<triangleright> \<Phi>)
           \<supseteq> { \<Gamma>, n \<turnstile> \<Psi> \<triangleright> (K sporadic \<tau>) # \<Phi>,
               K \<Up> n # K \<Down> n @ \<lfloor>\<tau>\<rfloor> # \<Gamma>, n \<turnstile> \<Psi> \<triangleright> \<Phi> }"
   by (simp add: operational_semantics_step.simps operational_semantics_elim.sporadic_e1 operational_semantics_elim.sporadic_e2)
 
-lemma Fnext_solve_sporadicon:
-  shows "\<F>\<^sub>n\<^sub>e\<^sub>x\<^sub>t (\<Gamma>, n \<turnstile> (K\<^sub>1 sporadic \<tau> on K\<^sub>2) # \<Psi> \<triangleright> \<Phi>)
+lemma Cnext_solve_sporadicon:
+  shows "\<C>\<^sub>n\<^sub>e\<^sub>x\<^sub>t (\<Gamma>, n \<turnstile> (K\<^sub>1 sporadic \<tau> on K\<^sub>2) # \<Psi> \<triangleright> \<Phi>)
           \<supseteq> { \<Gamma>, n \<turnstile> \<Psi> \<triangleright> (K\<^sub>1 sporadic \<tau> on K\<^sub>2) # \<Phi>,
               K\<^sub>1 \<Up> n # K\<^sub>2 \<Down> n @ \<tau> # \<Gamma>, n \<turnstile> \<Psi> \<triangleright> \<Phi> }"
   by (simp add: operational_semantics_step.simps operational_semantics_elim.sporadic_on_e1 operational_semantics_elim.sporadic_on_e2)
 
-lemma Fnext_solve_tagrel:
-  shows "\<F>\<^sub>n\<^sub>e\<^sub>x\<^sub>t (\<Gamma>, n \<turnstile> (tag-relation K\<^sub>1 = \<alpha> * K\<^sub>2 + \<beta>) # \<Psi> \<triangleright> \<Phi>)
+lemma Cnext_solve_tagrel:
+  shows "\<C>\<^sub>n\<^sub>e\<^sub>x\<^sub>t (\<Gamma>, n \<turnstile> (tag-relation K\<^sub>1 = \<alpha> * K\<^sub>2 + \<beta>) # \<Psi> \<triangleright> \<Phi>)
           \<supseteq> { (\<tau>\<^sub>v\<^sub>a\<^sub>r(K\<^sub>1, n) \<doteq> \<alpha> * \<tau>\<^sub>v\<^sub>a\<^sub>r(K\<^sub>2, n) + \<beta>) # \<Gamma>, n \<turnstile> \<Psi> \<triangleright> (tag-relation K\<^sub>1 = \<alpha> * K\<^sub>2 + \<beta>) # \<Phi> }"
   by (simp add: operational_semantics_step.simps operational_semantics_elim.tagrel_e)
 
-lemma Fnext_solve_tagrelgen:
-  shows "\<F>\<^sub>n\<^sub>e\<^sub>x\<^sub>t (\<Gamma>, n \<turnstile> (tag-relation \<langle>K\<^sub>1, K\<^sub>2\<rangle> \<in> R) # \<Psi> \<triangleright> \<Phi>)
+lemma Cnext_solve_tagrelgen:
+  shows "\<C>\<^sub>n\<^sub>e\<^sub>x\<^sub>t (\<Gamma>, n \<turnstile> (tag-relation \<langle>K\<^sub>1, K\<^sub>2\<rangle> \<in> R) # \<Psi> \<triangleright> \<Phi>)
           \<supseteq> { (\<langle>\<tau>\<^sub>v\<^sub>a\<^sub>r(K\<^sub>1, n), \<tau>\<^sub>v\<^sub>a\<^sub>r(K\<^sub>2, n)\<rangle> \<epsilon> R) # \<Gamma>, n \<turnstile> \<Psi> \<triangleright> (tag-relation \<langle>K\<^sub>1, K\<^sub>2\<rangle> \<in> R) # \<Phi> }"
   by (simp add: operational_semantics_step.simps operational_semantics_elim.tagrelgen_e)
 
-lemma Fnext_solve_implies:
-  shows "\<F>\<^sub>n\<^sub>e\<^sub>x\<^sub>t (\<Gamma>, n \<turnstile> (K\<^sub>1 implies K\<^sub>2) # \<Psi> \<triangleright> \<Phi>)
+lemma Cnext_solve_implies:
+  shows "\<C>\<^sub>n\<^sub>e\<^sub>x\<^sub>t (\<Gamma>, n \<turnstile> (K\<^sub>1 implies K\<^sub>2) # \<Psi> \<triangleright> \<Phi>)
           \<supseteq> { K\<^sub>1 \<not>\<Up> n # \<Gamma>, n \<turnstile> \<Psi> \<triangleright> (K\<^sub>1 implies K\<^sub>2) # \<Phi>,
               K\<^sub>1 \<Up> n # K\<^sub>2 \<Up> n # \<Gamma>, n \<turnstile> \<Psi> \<triangleright> (K\<^sub>1 implies K\<^sub>2) # \<Phi>}"
   by (simp add: operational_semantics_step.simps operational_semantics_elim.implies_e1 operational_semantics_elim.implies_e2)
 
-lemma Fnext_solve_timedelayed:
-  shows "\<F>\<^sub>n\<^sub>e\<^sub>x\<^sub>t (\<Gamma>, n \<turnstile> (K\<^sub>1 time-delayed by \<delta>\<tau> on K\<^sub>2 implies K\<^sub>3) # \<Psi> \<triangleright> \<Phi>)
+lemma Cnext_solve_timedelayed:
+  shows "\<C>\<^sub>n\<^sub>e\<^sub>x\<^sub>t (\<Gamma>, n \<turnstile> (K\<^sub>1 time-delayed by \<delta>\<tau> on K\<^sub>2 implies K\<^sub>3) # \<Psi> \<triangleright> \<Phi>)
           \<supseteq> { K\<^sub>1 \<not>\<Up> n # \<Gamma>, n \<turnstile> \<Psi> \<triangleright> (K\<^sub>1 time-delayed by \<delta>\<tau> on K\<^sub>2 implies K\<^sub>3) # \<Phi>,
               K\<^sub>1 \<Up> n # \<Gamma>, n \<turnstile> (K\<^sub>3 sporadic \<lfloor>\<tau>\<^sub>v\<^sub>a\<^sub>r(K\<^sub>2, n) \<oplus> \<delta>\<tau>\<rfloor> on K\<^sub>2) # \<Psi> \<triangleright> (K\<^sub>1 time-delayed by \<delta>\<tau> on K\<^sub>2 implies K\<^sub>3) # \<Phi> }"
   by (simp add: operational_semantics_step.simps operational_semantics_elim.timedelayed_e1 operational_semantics_elim.timedelayed_e2)
@@ -154,6 +146,7 @@ lemma empty_spec_reductions:
       using instant_i intro_part by auto
   qed
 
+(* To decide finite-satisfiability of TESL specifications *)
 inductive finite_SAT :: "config \<Rightarrow> bool" ("\<TTurnstile> _" 50) where
   finite_SAT_ax: "set (NoSporadic \<Phi>) = set \<Phi> \<Longrightarrow>
                     consistent_run \<Gamma> \<Longrightarrow>
