src/Denotational.thy
@@ -5,9 +5,9 @@ imports
 
 begin
 
-(**) section \<open>Denotational interpretation for atomic TESL formulae\<close> (**)
+section \<open>Denotational interpretation for atomic TESL formulae\<close>
 
-(* Denotational interpretation of TESL *)
+(* Denotational interpretation of TESL atomic formulae *)
 fun TESL_interpretation_atomic
     :: "TESL_atomic \<Rightarrow> run set" ("\<lbrakk> _ \<rbrakk>\<^sub>T\<^sub>E\<^sub>S\<^sub>L") where
     "\<lbrakk> K sporadic \<tau> \<rbrakk>\<^sub>T\<^sub>E\<^sub>S\<^sub>L =
@@ -31,7 +31,7 @@ fun TESL_interpretation_atomic
                  )
         }"
 
-(**) section \<open>Denotational interpretation for TESL formulae\<close> (**)
+section \<open>Denotational interpretation for TESL formulae\<close>
 
 fun TESL_interpretation :: "TESL_formula \<Rightarrow> run set" ("\<lbrakk>\<lbrakk> _ \<rbrakk>\<rbrakk>\<^sub>T\<^sub>E\<^sub>S\<^sub>L") where
     "\<lbrakk>\<lbrakk> [] \<rbrakk>\<rbrakk>\<^sub>T\<^sub>E\<^sub>S\<^sub>L = { _. True }"
@@ -41,7 +41,7 @@ lemma TESL_interpretation_homo:
   "\<lbrakk> \<phi> \<rbrakk>\<^sub>T\<^sub>E\<^sub>S\<^sub>L \<inter> \<lbrakk>\<lbrakk> \<Phi> \<rbrakk>\<rbrakk>\<^sub>T\<^sub>E\<^sub>S\<^sub>L = \<lbrakk>\<lbrakk> \<phi> # \<Phi> \<rbrakk>\<rbrakk>\<^sub>T\<^sub>E\<^sub>S\<^sub>L"
   by auto
 
-(***) subsection \<open>Fixpoint lemma\<close> (***)
+subsection \<open>Image interpretation lemma\<close>
 
 theorem TESL_interpretation_image:
   "\<lbrakk>\<lbrakk> \<Phi> \<rbrakk>\<rbrakk>\<^sub>T\<^sub>E\<^sub>S\<^sub>L = \<Inter> ((\<lambda>\<phi>. \<lbrakk> \<phi> \<rbrakk>\<^sub>T\<^sub>E\<^sub>S\<^sub>L) ` set \<Phi>)"
@@ -53,12 +53,10 @@ theorem TESL_interpretation_image:
     then show ?case by auto
   qed
 
-lemmas TESL_interpretation_cons_morph = TESL_interpretation_homo (*legacy *)
-lemmas TESL_interp_fixpoint = TESL_interpretation_image (*legacy *)
-(***) subsection \<open>Expansion law\<close> (***)
+subsection \<open>Expansion law\<close>
 text \<open>Similar to the expansion laws of lattices\<close>
 
-theorem TESL_interp_composition: (* modifier le nom homo_append *)
+theorem TESL_interp_homo_append:
   shows "\<lbrakk>\<lbrakk> \<Phi>\<^sub>1 @ \<Phi>\<^sub>2 \<rbrakk>\<rbrakk>\<^sub>T\<^sub>E\<^sub>S\<^sub>L = \<lbrakk>\<lbrakk> \<Phi>\<^sub>1 \<rbrakk>\<rbrakk>\<^sub>T\<^sub>E\<^sub>S\<^sub>L \<inter> \<lbrakk>\<lbrakk> \<Phi>\<^sub>2 \<rbrakk>\<rbrakk>\<^sub>T\<^sub>E\<^sub>S\<^sub>L"
   proof (induct \<Phi>\<^sub>1)
     case Nil
@@ -69,7 +67,7 @@ theorem TESL_interp_composition: (* modifier le nom homo_append *)
   qed
 
 
-(***) subsection \<open>Equational laws for TESL formulae denotationally interpreted\<close> (***)
+subsection \<open>Equational laws for TESL formulae denotationally interpreted\<close>
 
 lemma TESL_interp_assoc:
   shows "\<lbrakk>\<lbrakk> (\<Phi>\<^sub>1 @ \<Phi>\<^sub>2) @ \<Phi>\<^sub>3 \<rbrakk>\<rbrakk>\<^sub>T\<^sub>E\<^sub>S\<^sub>L = \<lbrakk>\<lbrakk> \<Phi>\<^sub>1 @ (\<Phi>\<^sub>2 @ \<Phi>\<^sub>3) \<rbrakk>\<rbrakk>\<^sub>T\<^sub>E\<^sub>S\<^sub>L"
@@ -77,23 +75,23 @@ lemma TESL_interp_assoc:
 
 lemma TESL_interp_commute:
   shows "\<lbrakk>\<lbrakk> \<Phi>\<^sub>1 @ \<Phi>\<^sub>2 \<rbrakk>\<rbrakk>\<^sub>T\<^sub>E\<^sub>S\<^sub>L = \<lbrakk>\<lbrakk> \<Phi>\<^sub>2 @ \<Phi>\<^sub>1 \<rbrakk>\<rbrakk>\<^sub>T\<^sub>E\<^sub>S\<^sub>L"
-  by (simp add: TESL_interp_composition inf_sup_aci(1))
+  by (simp add: TESL_interp_homo_append inf_sup_aci(1))
 
 lemma TESL_interp_left_commute:
   shows "\<lbrakk>\<lbrakk> \<Phi>\<^sub>1 @ (\<Phi>\<^sub>2 @ \<Phi>\<^sub>3) \<rbrakk>\<rbrakk>\<^sub>T\<^sub>E\<^sub>S\<^sub>L = \<lbrakk>\<lbrakk> \<Phi>\<^sub>2 @ (\<Phi>\<^sub>1 @ \<Phi>\<^sub>3) \<rbrakk>\<rbrakk>\<^sub>T\<^sub>E\<^sub>S\<^sub>L"
-  using TESL_interp_composition by auto
+  using TESL_interp_homo_append by auto
 
 lemma TESL_interp_idem:
   shows "\<lbrakk>\<lbrakk> \<Phi> @ \<Phi> \<rbrakk>\<rbrakk>\<^sub>T\<^sub>E\<^sub>S\<^sub>L = \<lbrakk>\<lbrakk> \<Phi> \<rbrakk>\<rbrakk>\<^sub>T\<^sub>E\<^sub>S\<^sub>L"
-  using TESL_interp_composition by auto
+  using TESL_interp_homo_append by auto
 
 lemma TESL_interp_left_idem:
   shows "\<lbrakk>\<lbrakk> \<Phi>\<^sub>1 @ (\<Phi>\<^sub>1 @ \<Phi>\<^sub>2) \<rbrakk>\<rbrakk>\<^sub>T\<^sub>E\<^sub>S\<^sub>L = \<lbrakk>\<lbrakk> \<Phi>\<^sub>1 @ \<Phi>\<^sub>2 \<rbrakk>\<rbrakk>\<^sub>T\<^sub>E\<^sub>S\<^sub>L"
-  using TESL_interp_composition by auto
+  using TESL_interp_homo_append by auto
 
 lemma TESL_interp_right_idem:
   shows "\<lbrakk>\<lbrakk> (\<Phi>\<^sub>1 @ \<Phi>\<^sub>2) @ \<Phi>\<^sub>2 \<rbrakk>\<rbrakk>\<^sub>T\<^sub>E\<^sub>S\<^sub>L = \<lbrakk>\<lbrakk> \<Phi>\<^sub>1 @ \<Phi>\<^sub>2 \<rbrakk>\<rbrakk>\<^sub>T\<^sub>E\<^sub>S\<^sub>L"
-  using TESL_interp_composition by auto
+  using TESL_interp_homo_append by auto
 
 lemmas TESL_interp_aci = TESL_interp_commute TESL_interp_assoc TESL_interp_left_commute TESL_interp_left_idem
 
@@ -114,12 +112,12 @@ lemma TESL_sem_decreases_head:
 
 lemma TESL_sem_decreases_tail:
   "\<lbrakk>\<lbrakk> \<Phi> \<rbrakk>\<rbrakk>\<^sub>T\<^sub>E\<^sub>S\<^sub>L \<supseteq> \<lbrakk>\<lbrakk> \<Phi> @ [\<phi>] \<rbrakk>\<rbrakk>\<^sub>T\<^sub>E\<^sub>S\<^sub>L"
-  by (simp add: TESL_interp_composition)
+  by (simp add: TESL_interp_homo_append)
 
 lemma TESL_interp_formula_stuttering:
   assumes bel: "\<phi> \<in> set \<Phi>"
   shows "\<lbrakk>\<lbrakk> \<phi> # \<Phi> \<rbrakk>\<rbrakk>\<^sub>T\<^sub>E\<^sub>S\<^sub>L = \<lbrakk>\<lbrakk> \<Phi> \<rbrakk>\<rbrakk>\<^sub>T\<^sub>E\<^sub>S\<^sub>L"
-  by (metis Int_subset_iff TESL_interp_composition TESL_interpretation.simps(2) bel in_set_conv_decomp_first subset_antisym subset_refl)
+  by (metis Int_subset_iff TESL_interp_homo_append TESL_interpretation.simps(2) bel in_set_conv_decomp_first subset_antisym subset_refl)
 
 lemma TESL_interp_decreases:
   shows "\<lbrakk>\<lbrakk> \<Phi> \<rbrakk>\<rbrakk>\<^sub>T\<^sub>E\<^sub>S\<^sub>L \<supseteq> \<lbrakk>\<lbrakk> \<phi> # \<Phi> \<rbrakk>\<rbrakk>\<^sub>T\<^sub>E\<^sub>S\<^sub>L"
@@ -143,9 +141,9 @@ lemma TESL_interp_set_lifting:
     have "set (remdups \<Phi>) = set (remdups \<Phi>')"
       by (simp add: assms)
     moreover have fxpnt\<Phi>: "\<Inter> ((\<lambda>\<phi>. \<lbrakk> \<phi> \<rbrakk>\<^sub>T\<^sub>E\<^sub>S\<^sub>L) ` set \<Phi>) = \<lbrakk>\<lbrakk> \<Phi> \<rbrakk>\<rbrakk>\<^sub>T\<^sub>E\<^sub>S\<^sub>L"
-      by (simp add: TESL_interp_fixpoint)
+      by (simp add: TESL_interpretation_image)
     moreover have fxpnt\<Phi>': "\<Inter> ((\<lambda>\<phi>. \<lbrakk> \<phi> \<rbrakk>\<^sub>T\<^sub>E\<^sub>S\<^sub>L) ` set \<Phi>') = \<lbrakk>\<lbrakk> \<Phi>' \<rbrakk>\<rbrakk>\<^sub>T\<^sub>E\<^sub>S\<^sub>L"
-      by (simp add: TESL_interp_fixpoint)
+      by (simp add: TESL_interpretation_image)
     moreover have "\<Inter> ((\<lambda>\<phi>. \<lbrakk> \<phi> \<rbrakk>\<^sub>T\<^sub>E\<^sub>S\<^sub>L) ` set \<Phi>) = \<Inter> ((\<lambda>\<phi>. \<lbrakk> \<phi> \<rbrakk>\<^sub>T\<^sub>E\<^sub>S\<^sub>L) ` set \<Phi>')"
       by (simp add: assms)
     ultimately show ?thesis using TESL_interp_remdups_absorb by auto
@@ -159,7 +157,7 @@ theorem TESL_interp_decreases_setinc:
     have "set (\<Phi> @ \<Phi>\<^sub>r) = set \<Phi>'" using incl decompose by blast
     moreover have "(set \<Phi>) \<union> (set \<Phi>\<^sub>r) = set \<Phi>'" using incl decompose by auto
     moreover have "\<lbrakk>\<lbrakk> \<Phi>' \<rbrakk>\<rbrakk>\<^sub>T\<^sub>E\<^sub>S\<^sub>L = \<lbrakk>\<lbrakk> \<Phi> @ \<Phi>\<^sub>r \<rbrakk>\<rbrakk>\<^sub>T\<^sub>E\<^sub>S\<^sub>L" using TESL_interp_set_lifting decompose by blast
-    moreover have "\<lbrakk>\<lbrakk> \<Phi> @ \<Phi>\<^sub>r \<rbrakk>\<rbrakk>\<^sub>T\<^sub>E\<^sub>S\<^sub>L = \<lbrakk>\<lbrakk> \<Phi> \<rbrakk>\<rbrakk>\<^sub>T\<^sub>E\<^sub>S\<^sub>L \<inter> \<lbrakk>\<lbrakk> \<Phi>\<^sub>r \<rbrakk>\<rbrakk>\<^sub>T\<^sub>E\<^sub>S\<^sub>L" by (simp add: TESL_interp_composition)
+    moreover have "\<lbrakk>\<lbrakk> \<Phi> @ \<Phi>\<^sub>r \<rbrakk>\<rbrakk>\<^sub>T\<^sub>E\<^sub>S\<^sub>L = \<lbrakk>\<lbrakk> \<Phi> \<rbrakk>\<rbrakk>\<^sub>T\<^sub>E\<^sub>S\<^sub>L \<inter> \<lbrakk>\<lbrakk> \<Phi>\<^sub>r \<rbrakk>\<rbrakk>\<^sub>T\<^sub>E\<^sub>S\<^sub>L" by (simp add: TESL_interp_homo_append)
     moreover have "\<lbrakk>\<lbrakk> \<Phi> \<rbrakk>\<rbrakk>\<^sub>T\<^sub>E\<^sub>S\<^sub>L \<supseteq> \<lbrakk>\<lbrakk> \<Phi> \<rbrakk>\<rbrakk>\<^sub>T\<^sub>E\<^sub>S\<^sub>L \<inter> \<lbrakk>\<lbrakk> \<Phi>\<^sub>r \<rbrakk>\<rbrakk>\<^sub>T\<^sub>E\<^sub>S\<^sub>L" by simp
     ultimately show ?thesis by simp
   qed
@@ -177,15 +175,14 @@ lemma TESL_interp_decreases_add_tail:
 lemma TESL_interp_absorb1:
   assumes incl: "set \<Phi>\<^sub>1 \<subseteq> set \<Phi>\<^sub>2"
   shows "\<lbrakk>\<lbrakk> \<Phi>\<^sub>1 @ \<Phi>\<^sub>2 \<rbrakk>\<rbrakk>\<^sub>T\<^sub>E\<^sub>S\<^sub>L = \<lbrakk>\<lbrakk> \<Phi>\<^sub>2 \<rbrakk>\<rbrakk>\<^sub>T\<^sub>E\<^sub>S\<^sub>L"
-  by (simp add: Int_absorb1 TESL_interp_decreases_setinc TESL_interp_composition incl)
+  by (simp add: Int_absorb1 TESL_interp_decreases_setinc TESL_interp_homo_append incl)
 
 lemma TESL_interp_absorb2:
   assumes incl: "set \<Phi>\<^sub>2 \<subseteq> set \<Phi>\<^sub>1"
   shows "\<lbrakk>\<lbrakk> \<Phi>\<^sub>1 @ \<Phi>\<^sub>2 \<rbrakk>\<rbrakk>\<^sub>T\<^sub>E\<^sub>S\<^sub>L = \<lbrakk>\<lbrakk> \<Phi>\<^sub>1 \<rbrakk>\<rbrakk>\<^sub>T\<^sub>E\<^sub>S\<^sub>L"
   using TESL_interp_absorb1 TESL_interp_commute incl by blast
 
-
-(***) subsection \<open>Some special cases\<close> (***)
+subsection \<open>Some special cases\<close>
 
 lemma NoSporadic_stable [simp]:
   shows "\<lbrakk>\<lbrakk> \<Phi> \<rbrakk>\<rbrakk>\<^sub>T\<^sub>E\<^sub>S\<^sub>L \<subseteq> \<lbrakk>\<lbrakk> NoSporadic \<Phi> \<rbrakk>\<rbrakk>\<^sub>T\<^sub>E\<^sub>S\<^sub>L"
@@ -206,4 +203,14 @@ lemma SporadicOn_sugar_atom:
 lemma SporadicOn_sugar:
   shows "\<lbrakk>\<lbrakk> (K sporadic \<lfloor>\<tau>\<rfloor> on K) # \<Phi> \<rbrakk>\<rbrakk>\<^sub>T\<^sub>E\<^sub>S\<^sub>L = \<lbrakk>\<lbrakk> (K sporadic \<tau>) # \<Phi> \<rbrakk>\<rbrakk>\<^sub>T\<^sub>E\<^sub>S\<^sub>L"
   by auto
+
+lemma Tagrel_affine_sugar:
+  shows "\<lbrakk> tag-relation K\<^sub>1 = \<alpha> * K\<^sub>2 + \<beta> \<rbrakk>\<^sub>T\<^sub>E\<^sub>S\<^sub>L = \<lbrakk> tag-relation \<langle>K\<^sub>1, K\<^sub>2\<rangle> \<in> (\<lambda>(\<tau>\<^sub>1, \<tau>\<^sub>2). \<tau>\<^sub>1 = \<alpha> * \<tau>\<^sub>2 + \<beta>) \<rbrakk>\<^sub>T\<^sub>E\<^sub>S\<^sub>L"
+  proof -
+    have "\<lbrakk> tag-relation \<langle>K\<^sub>1, K\<^sub>2\<rangle> \<in> (\<lambda>(\<tau>\<^sub>1, \<tau>\<^sub>2). \<tau>\<^sub>1 = \<alpha> * \<tau>\<^sub>2 + \<beta>) \<rbrakk>\<^sub>T\<^sub>E\<^sub>S\<^sub>L
+       = { \<rho>. \<forall>n::nat. (\<lambda>(\<tau>\<^sub>1, \<tau>\<^sub>2). \<tau>\<^sub>1 = \<alpha> * \<tau>\<^sub>2 + \<beta>) (time ((Rep_run \<rho>) n K\<^sub>1), time ((Rep_run \<rho>) n K\<^sub>2)) }"
+      by auto
+    then show ?thesis by auto
+  qed
+
 end
